\documentclass[12pt]{article}

\title{}
\author{Marci McBride}

\begin{document}
\maketitle 
        CSE 122 Homework 1
        \\ Problem 1: Show $1^2 + 2^2 + \ldots + n^2 = n(n+1)(2n+1)/6$
        \\
        \indent Base Case: $n = 1$
        \\\indent \indent $1^2 = 1$
        \\\indent \indent $1(1+1)(2(1)+1)/6=1 $
        \\\indent Assume:
        \\\indent \indent $1^2 + 2^2 + \ldots + k^2 = k(k+1)(2k+1)/6$
        \\\indent Show:
        \\\indent \indent $1^2 + 2^2 + \ldots + k^2 + (k+1)^2 = (k+1)(k+2)(2k+3)/6$
        \\\indent Proof:
        \\\indent \indent$1^2 + 2^2 + \ldots + k^2 + (k+1)^2  = [1^2 + 2^2 + \ldots + k^2 ] + (k+1)^2$
        \\\indent \indent$=[k(k+1)(2k+1)/6] + (k+1)^2$
        \\\indent \indent $=(2k^3+9k^2+13k+6)/6 $
        \\\indent \indent $=(k+1)(k+2)(2k+3)/6$
        \\\indent \indent $(k+1)(k+2)(2k+3)/6 =(k+1)(k+2)(2k+3)/6$
        \\\indent \indent TRUE
        \\
        \\Problem 2: Show  $1^3 + 2^3 + \ldots + n^3 = [n(n+1)/2]^2$
        \\\indent Base Case: $n = 1$
        \\\indent \indent $1^3 = 1 $
        \\\indent \indent $[1(1+1)/2]^2 =1$
        \\\indent Assume: 
        \\\indent \indent $1^3 + 2^3 + \ldots + k^3 = [k(k+1)/2]^2$
        \\\indent Show:
        \\\indent \indent $1^3 + 2^3 + \ldots + k^3 + (k+1)^3 = [(k+1)(k+2)/2]^2$
        \\\indent Proof:
        \\\indent \indent $[1^3 + 2^3 + \ldots + k^3] + (k+1)^3 = [(k+1)(k+2)/2]^2$
        \\\indent \indent $=[k(k+1)/2]^2+ (k+1)^3$
        \\\indent \indent$=(k^4+2k^3+k^2)/4 + (k^3+3k^2+3k+1)$
        \\\indent \indent$=(k^4+6k^3+13k^2+12k^4)/4$
        \\\indent \indent $[(k+1)(k+2)/2]^2=[(k+1)(k+2)/2]^2$
        \\\indent \indent TRUE 
        \\
        \\Problem 3: Show $1*1! + 2*2! + \ldots + n*n! = (n+1)! - 1 $
        \\\indent Base Case: $n=1$
        \\\indent \indent $1*1! = 1$
        \\\indent \indent $(1+1)! - 1 = 1$
        \\\indent Assume: 
        \\\indent \indent $1*1! + 2*2! + \ldots + k*k! = (k+1)! - 1 $
        \\\indent Show: 
        \\\indent \indent $1*1! + 2*2! + \ldots + k*k! + (k+1)*(k+1)! = (k+2)! - 1 $
        \\\indent Proof:
        \\\indent \indent $1*1! + 2*2! + \ldots + k*k! + (k+1)*(k+1)! = (k+2)! - 1 $
        \\\indent \indent $=[(k+1)! - 1] + (k+1)*(k+1)!$
        \\\indent \indent $=(k+1)! *(1+k+1) -1$
        \\\indent \indent $=(k+1)! *(k+2) -1$
        \\\indent \indent $=(k+2)!-1$
        \\\indent \indent $(k+2)!-1=(k+2)!-1$
        \\\indent \indent TRUE
        \\
        \\Problem 4: Show $ 2^n > n^2 $ when $n > 4$
        \\\indent Base Case: $n=5$
        \\\indent \indent $2^5 = 32$
        \\\indent \indent $5^2 = 25$
        \\\indent \indent $32>25$
        \\\indent Assume:
        \\\indent \indent $ 2^k > k^2 $ when $k > 4$
        \\\indent Show:
        \\\indent \indent $ 2^k + 2^{k+1} > (k+1)^2 $
        \\\indent Proof:
        \\\indent \indent $ 2^k + 2^{k+1} > (k+1)^2 $
        \\\indent \indent $ 2^k + 2^k*2 > k^2 + 2k+ 1 $
        \\\indent \indent TRUE
        \\
        \\Problem 5: Show 
        $1^3 + 3^3 + 5^3 + \ldots + (2n-1)^3 = n^2(2n^2-1) $
        \\\indent Base Case: $n=1$
        \\\indent \indent $(2(1)-1)^3=1$
        \\\indent \indent $1^2(2(1)^2-1)=1$
        \\\indent Assume:
        \\\indent \indent 
        $1^3 + 3^3 + 5^3 + \ldots + (2k-1)^3 = k^2(2k^2-1)$
        \\\indent Show:
        \\\indent \indent 
        $1^3 + 3^3 + 5^3 + \ldots + (2k-1)^3 + (2k+1)^3 = (k+1)^2(2(k+1)^2-1)$
        \\\indent Proof:
        \\\indent \indent
        $[1^3 + 3^3 + 5^3 + \ldots + (2k-1)^3 ]+ (2k+1)^3 = (k+1)^2(2(k+1)^2-1)$
        \\\indent \indent $=[k^2(2k^2-1)]+(2k+1)^3$
        \\\indent \indent $=2k^4-k^2+(8k^3+8k^2+2k+4k^2+4k+1)$
        \\\indent \indent $=2k^4+8k^3+11k^2+6k+1$
        \\\indent \indent $(k+1)^2(2(k+1)^2-1) = (k+1)^2(2(k+1)^2-1)$
        \\\indent \indent TRUE
        \\
        \\Problem 6: Show 
        \\\indent \indent $ \frac{1}{(1)(2)}+ \frac{1}{(2)(3)}+ \ldots + \frac{1}{n(n+1)} = \frac{n}{n+1}$
        \\\indent Base Case: $n=1$
        \\\indent \indent $\frac{1}{1(1+1)} =\frac{1}{2}$
        \\\indent \indent $\frac{1}{1+1} =\frac{1}{2}$
        \\\indent Assume:
        \\\indent \indent $ \frac{1}{(1)(2)}+ \frac{1}{(2)(3)}+ \ldots + \frac{1}{k(k+1)} = \frac{k}{k+1}$
        \\\indent Show:
        \\\indent \indent $ \frac{1}{(1)(2)}+ \frac{1}{(2)(3)}+ \ldots + \frac{1}{k(k+1)} + \frac{1}{(k+1)(k+2)} = \frac{k+1}{k+2}$
        \\\indent Proof:
        \\\indent \indent $ [\frac{1}{(1)(2)}+ \frac{1}{(2)(3)}+ \ldots + \frac{1}{k(k+1)}] + \frac{1}{(k+1)(k+2)} = \frac{k+1}{k+2}$
        \\\indent \indent $=[\frac{k}{k+1}] + \frac{1}{(k+1)(k+2)}$
        \\\indent \indent $=\frac{k(k+2)}{(k+1)(k+2)} + \frac{1}{(k+1)(k+2)} $
        \\\indent \indent $=\frac{k^2+2k+1}{(k+1)(k+2)}$
        \\\indent \indent $=\frac{(k+1)(k+1)}{(k+1)(k+2)}$
        \\\indent \indent $\frac{k+1}{k+2}= \frac{k+1}{k+2}$
        \\\indent \indent TRUE 
        \\
        \\Problem 7: Show 
        \\\indent \indent $ S= \sum\limits_{j=0}^n  ar^j= \frac{ar^{n+1}-a}{r-1} , r \neq 1 $
        \\\indent Base Case: $n=0$,$r=2$, $j=0$
        \\\indent \indent $a*2^0 = a $
        \\\indent \indent $\frac{a*2^{0+1}-a)}{2-1} = \frac{2a-a}{1} = a$
        \\\indent Assume:
        \\\indent \indent $ S= \sum\limits_{j=0}^k  ar^j= \frac{ar^{k+1}-a}{r-1} , r \neq 1 $
        \\\indent \indent $ar^0 +ar^1+ar^2+\ldots+ar^k=\frac{ar^{k+1}-a}{r-1}$
        \\\indent Show:
        \\\indent \indent $ar^0 +ar^1+ar^2+\ldots+ar^k+ar^{k+1}=\frac{ar^{k+2}-a}{r-1}$
        \\\indent Proof:
        \\\indent \indent $[ar^0 +ar^1+ar^2+\ldots+ar^k]+ar^{k+1}=\frac{ar^{k+2}-a}{r-1}$
        \\\indent \indent $ =[\frac{ar^{k+1}-a}{r-1}]+ar^{k+1}$
        \\\indent \indent $ =[\frac{ar^{k+1}-a+ar^{k+2}-ar^{k+1}}{r-1}]$
        \\\indent \indent $=\frac{ar^{k+2}-a}{r-1}$
        \\\indent \indent $\frac{ar^{k+2}-a}{r-1}=\frac{ar^{k+2}-a}{r-1}$
        \\\indent \indent TRUE
        \\
        \\Problem 8: Show
        \\ \indent \indent$ S= \sum\limits_{i=1}^{n+1} i*2^i = n* 2^{n+2} + 2$, for all integers $n \geq 0 $
        \\\indent Base Case: $n=0$
        \\\indent \indent $1*2^1 = 2$
        \\\indent \indent $0*2^{0+2}+2 =2 $
        \\\indent Assume:
        \\\indent \indent $(1*2^1)+(2*2^2)+ \ldots +(k*2^k)+((k+1)*2^{k+1}) = k*2^{k+2}+2$
        \\\indent Show:
        \\\indent \indent $(1*2^1)+(2*2^2)+ \ldots +(k*2^k)+((k+1)*2^{k+1})+((k+2)*2^{k+2}) = (k+1)*2^{k+3}+2$
        \\\indent Proof:
        \\\indent \indent $[(1*2^1)+(2*2^2)+ \ldots +(k*2^k)+((k+1)*2^{k+1})]+((k+2)*2^{k+2}) = (k+1)*2^{k+3}+2$        
        \\\indent \indent $=(k*2^{k+2}+2)+((k+2)*2^{k+2})$
        \\\indent \indent $=k*2^{k+2}+2+k*2^{k+2}+k*2^{k+3}$
        \\\indent \indent $=2^{k+3}*(k+1)+2$
        \\\indent \indent $(k+1)*2^{k+3}+2=(k+1)*2^{k+3}+2$
         \\\indent \indent TRUE 
\end{document}